proof/rejection_sampling/UniformSampling_Concrete_LF.ec
@@ -1,95 +1,15 @@
-require import W64_SchnorrExtract_ct.
-require import List Int AllCore.
+require import List Int AllCore Distr.
 
 from Jasmin require import JModel.
-(* require import Array1 WArray. *)
 
-
-(* SUBTRACTION LEAKAGES  *)
-op sub_prefix : leakages_t = 
-  [LeakFor (1, 32); LeakAddr []; LeakAddr [0]; LeakAddr []; 
-    LeakAddr []; LeakAddr [0]; LeakAddr [0]].
-
-op sub_step (i : int) : leakages_t = 
-  [LeakAddr [i] ; LeakAddr [] ; LeakAddr [] ; LeakAddr [i] ; 
-    LeakAddr [i] ].
-
-
-op sub_g (x : int) : leakages_t.
-axiom sub_g_comp_1 x : 1 <= x  => sub_g x = [].
-axiom sub_g_comp_2 x : 1 < x => sub_g x = sub_step (x-1) ++ sub_g (x - 1).
-
-op sub_f (x : int) : leakages_t = sub_g x ++ sub_prefix.
-
-
-lemma bn_subc_leakages start_l :
-   hoare [ M(Syscall).bn_subc : M.leakages = start_l ==> M.leakages = sub_f 32 ++ start_l ].
-proof. 
-proc.
-sp.  elim*. progress.
-conseq (_: M.leakages = sub_prefix ++ start_l /\ i = 1 ==> _).
-progress.
-while (0 < i /\ i <= 32 /\ M.leakages = sub_f i ++ start_l).
-wp.  skip.  progress. 
-simplify. smt(). smt(). rewrite /sub_f. rewrite (sub_g_comp_2 (i{hr} +1)).  smt(). simplify. rewrite /sub_step. simplify. auto.
-skip. progress. rewrite /sub_f.  rewrite sub_g_comp_1. auto. auto.
-smt().
-qed.
-
-
-(* COPY LEAKAGES  *)
-op copy_prefix : leakages_t = LeakFor (0, 32) :: LeakAddr [] ::[].
-op copy_step (i : int) : leakages_t = LeakAddr [i] :: LeakAddr [] :: LeakAddr [i] :: [].
-
-op copy_g (x : int) : leakages_t.
-axiom copy_g_comp_1 x : 0 <= x  => copy_g x = [].
-axiom copy_g_comp_2 x : 0 < x => copy_g x = copy_step (x-1) ++ copy_g (x - 1).
-
-op copy_f (x : int) : leakages_t = copy_g x ++ copy_prefix.
-
-lemma bn_copy_leakages start_l :
-   hoare [ M(Syscall).bn_copy : M.leakages = start_l ==> M.leakages = copy_f 32 ++ start_l ].
-proof. 
-proc.
-sp.  elim*. progress.
-conseq (_: M.leakages = copy_prefix ++ start_l /\ i = 0 ==> _).
-progress.
-while (0 <= i /\ i <= 32 /\ M.leakages = copy_f i ++ start_l).
-wp.  skip.  progress. 
-simplify. smt(). smt(). rewrite /copy_f. rewrite (copy_g_comp_2 (i{hr} +1)).  smt(). simplify. rewrite /copy_step. simplify. auto.
-skip. progress. rewrite /copy_f.  rewrite copy_g_comp_1. auto. auto. 
-smt().
-qed.
-
-
-
-(* set0 LEAKAGES  *)
-op set0_prefix : leakages_t = LeakFor (0, 32) :: LeakAddr [] :: [].
-op set0_step (i : int) : leakages_t = LeakAddr [i] :: LeakAddr [] :: [].
-
-op set0_g (x : int) : leakages_t.
-axiom set0_g_comp_1 x : 0 <= x  => set0_g x = [].
-axiom set0_g_comp_2 x : 0 < x => set0_g x = set0_step (x-1) ++ set0_g (x - 1).
-
-op set0_f (x : int) : leakages_t = set0_g x ++ set0_prefix.
-
-lemma bn_set0_leakages start_l :
-   hoare [ M(Syscall).bn_set0 : M.leakages = start_l ==> M.leakages = set0_f 32 ++ start_l ].
-proof. 
-proc.
-sp.  elim*. progress.
-conseq (_: M.leakages = set0_prefix ++ start_l /\ i = 0 ==> _).
-progress. rewrite /set0_prefix.
-while (0 <= i /\ i <= 32 /\ M.leakages = set0_f i ++ start_l).
-wp.  skip.  progress. 
-simplify. smt(). smt(). rewrite /set0_f. rewrite (set0_g_comp_2 (i{hr} +1)).  smt(). simplify. rewrite /set0_step. simplify. auto.
-skip. progress. rewrite /set0_f.  rewrite set0_g_comp_1. auto. auto. 
-smt().
-qed.
-
+require import AuxLemmas.
+require import Ops_LeakageAnalysis.
 
 
 (* SAMPLING LEAKAGES  *)
+require import W64_SchnorrExtract_ct.
+module M1 = W64_SchnorrExtract_ct.M(W64_SchnorrExtract_ct.Syscall).
+
 op samp_prefix : leakages_t = 
   LeakCond (! set0_64_.`2) :: LeakAddr [] :: LeakAddr [] :: (set0_f 32 ++
                                                            [LeakAddr [];
@@ -100,15 +20,13 @@ op samp_step (i : int) : leakages_t = LeakCond true :: LeakAddr [] :: LeakAddr [
                                                                 LeakAddr [] :: 
                                                                 LeakAddr [] :: [])) .
  
-
-axiom samp_g_comp_1 x : 0 <= x  => samp_g x = [].
-axiom samp_g_comp_2 x : 0 < x => samp_g x = samp_step (x-1) ++ samp_g (x - 1).
-
+axiom samp_g_comp_1 x : x <= 0 => samp_g x = [].
+axiom samp_g_comp_2 x : 0 <  x  => samp_g x = samp_step (x-1) ++ samp_g (x - 1).
 
 op samp_suffix : leakages_t = 
- LeakCond false :: LeakAddr [] :: LeakAddr []  :: (
-sub_f 32 ++
-LeakAddr [] :: (copy_f 32 ++ LeakAddr [] :: LeakAddr [] :: [])).
+ LeakCond false :: LeakAddr [] :: LeakAddr [] 
+   :: (sub_f 32 ++ LeakAddr [] :: 
+      (copy_f 32 ++ LeakAddr [] :: LeakAddr [] :: [])).
 
 op samp_f (x : int) : leakages_t = samp_g x ++ samp_prefix.
 op samp_t (x : int) : leakages_t = samp_suffix ++ samp_f (x - 1).
@@ -116,9 +34,9 @@ op samp_t (x : int) : leakages_t = samp_suffix ++ samp_f (x - 1).
 axiom samp_t_inj : injective samp_t.
 
 
-
-lemma rsample_leakages :
-   hoare [ M(Syscall).rsample : M.leakages = [] ==> M.leakages = samp_t res.`1].
+lemma rsample_leakages1 :
+  hoare [ M(Syscall).rsample : M.leakages = [] 
+     ==> M.leakages = samp_t res.`1].
 proc.
 seq 17 :  (M.leakages = samp_prefix /\ i = 0  /\ cf = false ).
 wp. ecall (bn_set0_leakages M.leakages). wp. skip. progress.  
@@ -140,124 +58,58 @@ auto. rewrite /samp_prefix. auto.
 rewrite H2. rewrite H. auto.
 auto.
 qed.
-    
-
-require import W64_SchnorrExtract.
-module M1 = W64_SchnorrExtract_ct.M(W64_SchnorrExtract_ct.Syscall).
-module M2 = W64_SchnorrExtract.M(W64_SchnorrExtract.Syscall).  
-
-lemma aaaa :
-  equiv  [ M1.bn_set0 ~ M2.bn_set0 
-    : ={arg} ==> ={res}  ].
-proc. 
-while (={a,i}). wp. skip. progress. wp.  skip. progress. qed.
-
-  
-lemma aaa :
-  equiv  [ M1.rsample ~ M2.rsample 
-    : ={arg} ==> ={res}  ].
-proof. proc.  sim. call aaaa. wp.  skip. progress. qed.
-
-require import Ring_ops_proof.
-require import Ring_ops_spec.
-require import UniformSampling_Abstract.
-require import UniformSampling_Concrete.
 
 
-
-equiv rsample_cspec2:
- M1.rsample ~ CSpecFp.rsample:
-  W64xN.valR byte_z{1} = a{2}
-  ==> W64xN.valR res{1}.`2 = res{2}.`2 /\ res{1}.`1 = res{2}.`1.
-transitivity M2.rsample 
- (={arg} ==> ={res})
- (W64xN.valR byte_z{1} = a{2}
-  ==> W64xN.valR res{1}.`2 = res{2}.`2 /\ res{1}.`1 = res{2}.`1).
-progress. smt(). progress.
-conseq aaa. 
-conseq rsample_cspec.
-qed.
-
-import W64xN.
-require import Distr.
-
-lemma samew a &m : 0%r < mu D (RSP (valR a)) =>
-  Pr[ M1.rsample(a) @ &m : true  ] = 1%r.
-progress.
-rewrite - (rsample_lossless (W64xN.valR a) &m _). auto. 
-byequiv.
-conseq rsample_cspec2. progress. progress. smt().
-qed.
-
-
-lemma sameww a &m : 
-  Pr[ M1.rsample(a) @ &m : true  ] = if 0%r < mu D (RSP (valR a)) then 1%r else 0%r.
-case (0%r < mu D (RSP (valR a))). move => pos. 
-rewrite - (rsample_lossless (W64xN.valR a) &m _). auto. 
-byequiv.
-conseq rsample_cspec2. progress. progress. smt().
-move => neg.
-have -> : Pr[M1.rsample(a) @ &m : true] = Pr[CSpecFp.rsample(W64xN.valR a) @ &m : true].
-byequiv. conseq rsample_cspec2. auto. auto. auto.
-print rsample_lossless0.
-apply (rsample_lossless0 (W64xN.valR a) &m (fun _ => true)).  smt().
-qed.
-
-
-
-
-lemma zzz a i x &m : 
-  Pr[ M1.rsample(a) @ &m : res = (i,x)  ]
-   =   Pr[ CSpecFp.rsample(W64xN.valR a) @ &m : res = (i, W64xN.valR x)  ].
-byequiv.
-conseq rsample_cspec2. progress. progress. smt().
-smt(@W64xN). auto. auto.
-qed.
-
-
-lemma qq' a  &m : (glob M1){m} = [] =>
+lemma rsample_leakages2 a  &m : (glob M1){m} = [] =>
   Pr[ M1.rsample(a) @ &m : M1.leakages <> samp_t res.`1 ] = 0%r.
 progress. byphoare (_: glob M1 = [] ==> _).
 hoare. simplify.
-conseq rsample_leakages. auto. auto. auto.
+conseq rsample_leakages1. auto. auto. auto.
 qed.
 
-lemma qq a l x &m : (glob M1){m} = [] => 
+
+lemma rsample_leakages3 a l x &m : (glob M1){m} = [] =>
   Pr[ M1.rsample(a) @ &m : M1.leakages = l  /\ res.`2 = x ]
   = Pr[ M1.rsample(a) @ &m : l = samp_t res.`1 /\ res.`2 = x  ].
-move => m1p.
-have pr1 :  Pr[ M1.rsample(a) @ &m : M1.leakages = samp_t res.`1   ] = b2r (0%r < mu D (RSP (valR a))).
-rewrite - (sameww a &m).   auto.
-  have ->: Pr[M1.rsample(a) @ &m : true] 
-   = Pr[M1.rsample(a) @ &m : M1.leakages = samp_t res.`1 ] + Pr[M1.rsample(a) @ &m : M1.leakages <> samp_t res.`1  ]. rewrite Pr[mu_split (M1.leakages = samp_t res.`1) ]. simplify. auto. rewrite (qq' a &m). auto.
-simplify. auto.
-have pr2 :  Pr[ M1.rsample(a) @ &m : M1.leakages <> samp_t res.`1   ] = 0%r.
-byphoare (_:(glob M1){m} = (glob M1) ==> _). 
-hoare. simplify.
-conseq rsample_leakages. smt(). progress. auto.
-have -> :   Pr[ M1.rsample(a) @ &m : M1.leakages = l /\ res.`2 = x  ]
- = Pr[ M1.rsample(a) @ &m : M1.leakages = samp_t res.`1 /\ M1.leakages = l /\ res.`2 = x ].
-rewrite Pr[mu_split (M1.leakages = samp_t res.`1) ].
-  have -> : Pr[M1.rsample(a) @ &m :
-   (M1.leakages = l /\ res.`2 = x) /\ M1.leakages <> samp_t res.`1] = 0%r. smt(@Distr). 
-   simplify. rewrite Pr[mu_eq]. progress. auto. 
-have -> : Pr[M1.rsample(a) @ &m : l = samp_t res.`1 /\ res.`2 = x] 
-  = Pr[M1.rsample(a) @ &m : l = samp_t res.`1 /\ M1.leakages = samp_t res.`1 /\ res.`2 = x  ].
-rewrite Pr[mu_split (M1.leakages = samp_t res.`1) ].
-  have -> : Pr[M1.rsample(a) @ &m :
-   (l = samp_t res.`1 /\ res.`2 = x) /\ M1.leakages <> samp_t res.`1] = 0%r. smt(@Distr).  auto. 
-   simplify. rewrite Pr[mu_eq]. progress. auto. 
-rewrite Pr[mu_eq]. progress. auto.
+move => H.
+have ->: Pr[ M1.rsample(a) @ &m : l = samp_t res.`1 /\ res.`2 = x ]
+ = Pr[ M1.rsample(a) @ &m : l = samp_t res.`1 /\ res.`2 = x /\ M1.leakages = samp_t res.`1  ].
+  have -> : Pr[M1.rsample(a) @ &m : l = samp_t res.`1 /\ res.`2 = x]
+   = Pr[M1.rsample(a) @ &m : l = samp_t res.`1 /\ res.`2 = x /\ M1.leakages = samp_t res.`1]
+   + Pr[M1.rsample(a) @ &m : l = samp_t res.`1 /\ res.`2 = x /\ M1.leakages <> samp_t res.`1].
+   rewrite Pr[mu_split (M1.leakages = samp_t res.`1)]. smt(). 
+  have ->: Pr[M1.rsample(a) @ &m :
+   l = samp_t res.`1 /\ res.`2 = x /\ M1.leakages <> samp_t res.`1] = 0%r.
+    have : Pr[M1.rsample(a) @ &m :
+       l = samp_t res.`1 /\ res.`2 = x /\ M1.leakages <> samp_t res.`1]
+     <= Pr[ M1.rsample(a) @ &m : M1.leakages <> samp_t res.`1 ]. smt(@Distr).
+    rewrite (rsample_leakages2 a &m). auto. smt(@Distr). 
+auto.
+have -> : Pr[ M1.rsample(a) @ &m : l = samp_t res.`1 /\ res.`2 = x /\ M1.leakages = samp_t res.`1  ]
+ = Pr[ M1.rsample(a) @ &m : res.`2 = x /\  l = M1.leakages /\ M1.leakages = samp_t res.`1  ].
+rewrite Pr[mu_eq]. move => &hr. split.  smt().  smt(). auto.
+have -> : Pr[ M1.rsample(a) @ &m : res.`2 = x /\ l = M1.leakages /\ M1.leakages = samp_t res.`1  ]
+ = Pr[ M1.rsample(a) @ &m :  l = M1.leakages /\ res.`2 = x ].
+  have : Pr[ M1.rsample(a) @ &m :  l = M1.leakages /\ res.`2 = x ] 
+   = Pr[ M1.rsample(a) @ &m :  l = M1.leakages /\ res.`2 = x /\ M1.leakages = samp_t res.`1  ]
+   + Pr[ M1.rsample(a) @ &m :  l = M1.leakages /\ res.`2 = x /\ M1.leakages <> samp_t res.`1  ].
+ rewrite Pr[mu_split (M1.leakages = samp_t res.`1 )]. smt().
+   have : Pr[ M1.rsample(a) @ &m :  l = M1.leakages /\ res.`2 = x /\ M1.leakages <> samp_t res.`1  ]
+    = 0%r.
+     have : Pr[ M1.rsample(a) @ &m :  l = M1.leakages /\ res.`2 = x /\ M1.leakages <> samp_t res.`1  ] 
+         <= Pr[ M1.rsample(a) @ &m : M1.leakages <> samp_t res.`1 ].
+       rewrite Pr[mu_sub]. auto. auto.
+    rewrite (rsample_leakages2 a &m). auto. smt(@Distr).
+    move => h. rewrite h. simplify. progress. rewrite H0.
+rewrite Pr[mu_eq]. smt(). auto. 
+rewrite Pr[mu_eq]. smt(). auto.
 qed.
 
-require import AuxLemmas.
 
-
-    
-lemma qqq a x l &m : (glob M1){m} = [] => (* 0%r < mu D (RSP (valR a)) => *)
-  Pr[ M1.rsample(a) @ &m : M1.leakages = l  /\ res.`2 = x  ]
+lemma rsample_leakages_inv a x l &m : (glob M1){m} = [] 
+ => Pr[ M1.rsample(a) @ &m : M1.leakages = l /\ res.`2 = x  ]
   = Pr[ M1.rsample(a) @ &m :  (inv (-1) samp_t) l = res.`1  /\ res.`2 = x  ].
-move => ic (* ic' *). rewrite  (qq a  l x &m). auto. auto.
+move => ic (* ic' *). rewrite  (rsample_leakages3 a l x &m). auto. auto.
 simplify. 
 have -> : 
   Pr[M1.rsample(a) @ &m :
@@ -298,8 +150,48 @@ auto.
 qed.
 
 
+require import W64_SchnorrExtract.
+module M2 = W64_SchnorrExtract.M(W64_SchnorrExtract.Syscall).  
 
-lemma ph_l5''_var &m a : Pr[M1.rsample(a) @ &m : res.`1 <= 0 ] = 0%r.
+lemma M1_M2_rsample :
+  equiv  [ M1.rsample ~ M2.rsample 
+    : ={arg} ==> ={res}  ].
+proof. proc.  sim. 
+call (_:true). 
+wp. while (={a,i}). wp.  skip. progress. wp. skip. progress.
+wp.  skip. progress. qed.
+
+
+require import Ring_ops_proof.
+require import Ring_ops_spec.
+require import UniformSampling_Abstract.
+require import UniformSampling_Concrete.
+
+
+equiv rsample_cspec_equiv:
+ M1.rsample ~ CSpecFp.rsample:
+  W64xN.valR byte_z{1} = a{2}
+  ==> W64xN.valR res{1}.`2 = res{2}.`2 /\ res{1}.`1 = res{2}.`1.
+transitivity M2.rsample 
+ (={arg} ==> ={res})
+ (W64xN.valR byte_z{1} = a{2}
+  ==> W64xN.valR res{1}.`2 = res{2}.`2 /\ res{1}.`1 = res{2}.`1).
+progress. smt(). progress.
+conseq M1_M2_rsample. 
+conseq rsample_cspec.
+qed.
+
+
+lemma rsample_cspec_pr a i x &m : 
+  Pr[ M1.rsample(a) @ &m : res = (i,x)  ]
+   = Pr[ CSpecFp.rsample(W64xN.valR a) @ &m : res = (i, W64xN.valR x)  ].
+byequiv.
+conseq rsample_cspec_equiv. progress. progress. smt().
+smt(@W64xN). auto. auto.
+qed.
+
+
+lemma rsample_index_pos &m a : Pr[M1.rsample(a) @ &m : res.`1 <= 0 ] = 0%r.
 byphoare (_: arg = a ==> _);auto. hoare.
 proc.  simplify.
 unroll 18. rcondt 18. wp. wp. 
@@ -312,27 +204,7 @@ call (_:true). auto. wp.
 call (_:true). auto. wp. skip. smt().
 qed.
 
-
-
-
-op h a : real = 1%r/(valR a)%r. 
-
-
-lemma leakfree2 &m x a: 
- Pr[ M1.rsample(a) @ &m : res.`2 = x ] 
-  = if (valR a <= valR x) then 0%r else h a.    
-proof. 
- have ->: Pr[ M1.rsample(a) @ &m : res.`2 = x ] =
-  Pr[ CSpecFp.rsample(W64xN.valR a) @ &m : res.`2 =  W64xN.valR x ].
-  byequiv. conseq rsample_cspec2. auto. 
-progress. rewrite - H. auto. smt(@W64xN). auto. auto.
-rewrite /h.
-case: (valR a <= valR x). move => alx.
-rewrite rsample_pr_out. smt(). auto.
-move => a_less_x.
-rewrite rsample_uni. smt(@W64xN).
-smt(@W64xN). smt(). auto.
-qed.
+import W64xN.
 
 
 op g a l : real 
@@ -344,13 +216,13 @@ op g a l : real
 lemma leakfree1 &m x a l: (glob M1){m} = [] 
   => Pr[ M1.rsample(a) @ &m : M1.leakages = l  /\ res.`2 = x  ] = if (valR a <= valR x) then 0%r else (g a l).
       progress.
-   rewrite  (qqq a x l &m);auto.
+   rewrite  (rsample_leakages_inv a x l &m);auto.
 case (inv (-1) samp_t l <= 0). 
 move => q. rewrite /g. rewrite q.  simplify. 
   have : Pr[M1.rsample(a) @ &m :
    inv (-1) samp_t l = res.`1 /\ res.`2 = x] 
     <= Pr[M1.rsample(a) @ &m : res.`1 <= 0 ]. simplify. rewrite Pr[mu_sub]. smt().
-   auto. smt(ph_l5''_var @Distr).
+   auto. smt(rsample_index_pos @Distr).
 move => q.
 have -> : 
  Pr[M1.rsample(a) @ &m :
@@ -358,7 +230,7 @@ have -> :
   = Pr[M1.rsample(a) @ &m :
    res = (inv (-1) samp_t l , x) ]. rewrite Pr[mu_eq]. smt(). auto.
 case (valR x < valR a) => case1.
-rewrite zzz.
+rewrite rsample_cspec_pr.
 rewrite rsample_pr.   smt().
 rewrite /RSP. auto.
 rewrite /z. 
@@ -370,11 +242,28 @@ have : Pr[W64_SchnorrExtract_ct.M(W64_SchnorrExtract_ct.Syscall).rsample(a) @ &m
    res.`2 = x] = 0%r.
   have -> : Pr[W64_SchnorrExtract_ct.M(W64_SchnorrExtract_ct.Syscall).rsample(a) @ &m :
      res.`2 =  x] = Pr[ CSpecFp.rsample(W64xN.valR a) @ &m : res.`2 =  W64xN.valR x ].
-  byequiv. conseq rsample_cspec2. auto. progress. rewrite H0.  auto.  smt(@W64xN). auto. auto.
+  byequiv. conseq rsample_cspec_equiv. auto. progress. rewrite H0.  auto.  smt(@W64xN). auto. auto.
   apply rsample_pr_out. auto.
 smt(@Distr).
 qed.
 
+op h a : real = 1%r/(valR a)%r. 
+
+lemma leakfree2 &m x a: 
+ Pr[ M1.rsample(a) @ &m : res.`2 = x ] 
+  = if (valR a <= valR x) then 0%r else h a.    
+proof. 
+ have ->: Pr[ M1.rsample(a) @ &m : res.`2 = x ] =
+  Pr[ CSpecFp.rsample(W64xN.valR a) @ &m : res.`2 =  W64xN.valR x ].
+  byequiv. conseq rsample_cspec_equiv. auto. 
+progress. rewrite - H. auto. smt(@W64xN). auto. auto.
+rewrite /h.
+case: (valR a <= valR x). move => alx.
+rewrite rsample_pr_out. smt(). auto.
+move => a_less_x.
+rewrite rsample_uni. smt(@W64xN).
+smt(@W64xN). smt(). auto.
+qed.
 
 op f a l = h a / g a l.
 
