proof/rejection_sampling/Commitment_LF.ec
@@ -1,0 +1,249 @@
+require import List Int AllCore Distr.
+
+from Jasmin require import JModel.
+
+require import AuxLemmas.
+require import Ops_LeakageAnalysis.
+
+
+(* SAMPLING LEAKAGES  *)
+require import W64_SchnorrExtract_ct.
+module M1 = W64_SchnorrExtract_ct.M(W64_SchnorrExtract_ct.Syscall).
+
+op commitment_prefix : leakages_t.
+op commitment_g (x : int) : leakages_t.
+op commitment_step (i : int) : leakages_t.
+ 
+axiom commitment_g_comp_1 x : x <= 0 => commitment_g x = [].
+axiom commitment_g_comp_2 x : 0 <  x  => commitment_g x = commitment_step (x-1) ++ commitment_g (x - 1).
+
+op commitment_suffix : leakages_t.
+
+op commitment_f (x : int) : leakages_t = commitment_g x ++ commitment_prefix.
+op commitment_t (x : int) : leakages_t = commitment_suffix ++ commitment_f (x - 1).
+
+axiom commitment_t_inj : injective commitment_t.
+
+
+lemma commitment_leakages1 :
+  hoare [ M(Syscall).commitment_indexed : M.leakages = [] 
+     ==> M.leakages = commitment_t res.`1].
+admitted.
+
+lemma commitment_leakages2 &m : (glob M1){m} = [] =>
+  Pr[ M1.commitment_indexed() @ &m : M1.leakages <> commitment_t res.`1 ] = 0%r.
+admitted.
+
+lemma commitment_leakages3 l x &m : (glob M1){m} = [] =>
+  Pr[ M1.commitment_indexed() @ &m : M1.leakages = l  /\ res.`2 = x ]
+  = Pr[ M1.commitment_indexed() @ &m : l = commitment_t res.`1 /\ res.`2 = x ].
+admitted.
+
+lemma commitment_leakages_inv x l &m : (glob M1){m} = [] 
+ => Pr[ M1.commitment_indexed() @ &m : M1.leakages = l /\ res.`2 = x  ]
+  = Pr[ M1.commitment_indexed() @ &m :  (inv (-1) commitment_t) l = res.`1  /\ res.`2 = x  ].
+admitted.
+
+require import W64_SchnorrExtract.
+module M2 = W64_SchnorrExtract.M(W64_SchnorrExtract.Syscall).  
+
+lemma M1_M2_commitment :
+  equiv  [ M1.commitment_indexed ~ M2.commitment_indexed
+    : ={arg} ==> ={res}  ].
+admitted.
+
+require import Ring_ops_proof.
+require import Ring_ops_spec.
+require import UniformSampling_Abstract.
+require import UniformSampling_Concrete.
+
+require Constants.
+
+require import IntDiv.
+require MontgomeryLadder_Concrete.
+require import ConstantsValidation.
+
+clone import MontgomeryLadder_Concrete as MLC with op Zp.p <- Constants.p.
+
+equiv commitment_rsample_equiv:
+ M2.commitment_indexed ~ M2.rsample:
+   Constants.q = W64xN.valR byte_z{2}
+  ==> res{1}.`3 = res{2}.`2 /\ res{1}.`1 = res{2}.`1.
+proc*.
+inline M2.commitment_indexed. 
+wp. call {1} (_:true ==> true).  admit.
+seq 10 0 : ( exp_order{1} =  byte_z{2}). 
+call {1} Constants.bn_set_bp_correct.
+call {1} Constants.bn_set_g_correct.
+call {1} Constants.bn_set_p_correct.
+call {1} Constants.bn_set_q_correct.
+wp. skip. progress. smt.
+simplify.
+call (_:true). sim. skip. auto.
+qed.
+equiv rsample_cspec_equiv:
+ M1.commitment_indexed ~ CSpecFp.rsample:
+   Constants.q = a{2}
+  ==> W64xN.valR res{1}.`3 = res{2}.`2 /\ res{1}.`1 = res{2}.`1.
+transitivity M2.commitment_indexed 
+ (={arg} ==> ={res})
+ (Constants.q = a{2}
+  ==> W64xN.valR res{1}.`3 = res{2}.`2 /\ res{1}.`1 = res{2}.`1).
+auto. auto.
+conseq M1_M2_commitment. 
+transitivity M2.rsample
+  (Constants.q = W64xN.valR byte_z{2}
+  ==> res{1}.`3 = res{2}.`2 /\ res{1}.`1 = res{2}.`1)
+  (W64xN.valR byte_z{1} = a{2}
+  ==> W64xN.valR res{1}.`2 = res{2}.`2 /\ res{1}.`1 = res{2}.`1).
+progress. exists (W64xN.R.bn_ofint Constants.q).
+split. 
+rewrite W64xN.R.bnk_ofintK. auto. admit.
+rewrite W64xN.R.bnk_ofintK. auto. admit.
+smt().
+conseq commitment_rsample_equiv. 
+conseq rsample_cspec.
+qed.
+
+
+lemma commitment_cspec_pr1 (i  : int) x &m : 
+  Pr[ M1.commitment_indexed() @ &m : res.`1 = i /\ res.`3 = x ]
+   = Pr[ CSpecFp.rsample(Constants.q) @ &m : res = (i, W64xN.valR x)  ].
+byequiv.
+conseq rsample_cspec_equiv. progress. progress. smt().
+smt(@W64xN). auto. auto.
+smt(@W64xN).
+auto. auto.
+qed.
+
+
+lemma val_congr a b :  
+  W64xN.valR a = W64xN.valR b => a = b.
+smt(@W64xN).
+qed.
+
+
+lemma val_congr2N a b :  
+  W64x2N.valR a = W64x2N.valR b => a = b.
+smt(@W64x2N).
+qed.
+
+lemma commitment_cspec_pr2 &m :
+  Pr[ M1.commitment_indexed() @ &m : res.`2 <> W64xN.R.bn_ofint (Constants.g ^ (W64xN.valR res.`3) %% Constants.p) ] = 0%r.
+have -> : Pr[ M1.commitment_indexed() @ &m : res.`2 <> W64xN.R.bn_ofint (Constants.g ^ (W64xN.valR res.`3) %% Constants.p) ] 
+ = Pr[ M2.commitment_indexed() @ &m : res.`2 <> W64xN.R.bn_ofint (Constants.g ^ (W64xN.valR res.`3) %% Constants.p) ].
+byequiv. conseq M1_M2_commitment. auto. auto.
+byphoare. hoare.
+simplify. proc.
+simplify.
+seq 11 : (W64xN.valR exp_order = Constants.q
+       /\ W64xN.valR group_order = Constants.p
+       /\ W64xN.valR group_generator = Constants.g
+       /\ barrett_parameter = R).
+call (_:true).  auto.
+call Constants.bn_set_bp_correct_hoare.
+call Constants.bn_set_g_correct_hoare.
+call Constants.bn_set_p_correct_hoare.
+call Constants.bn_set_q_correct_hoare.
+wp. skip. progress. apply (val_congr2N result2 R). rewrite H2.
+rewrite /R.
+rewrite W64x2N.R.bn_ofintK.
+rewrite /Ri. 
+rewrite - bp_correct.
+rewrite nasty_id.
+have : Constants.bp < W64x2N.modulusR. auto.
+smt(@IntDiv).
+exists* barrett_parameter, group_order, group_generator, secret_power.
+elim*. move => bp p g r.
+call (bn_expm_correct_hoare bp p g r).
+skip. progress. rewrite H1. auto.
+apply val_congr.
+rewrite H4. rewrite  H1.
+rewrite W64xN.R.bn_ofintK.
+pose x := Constants.g ^ (W64xN.valR secret_power{hr}).
+have : 0 <= Constants.p < W64xN.modulusR. auto.
+smt(@IntDiv). 
+auto.
+auto.
+qed.
+
+lemma commitment_cspec_pr3 i x &m :
+  Pr[ M1.commitment_indexed() @ &m : res.`1 = i /\ (res.`2, res.`3) = (W64xN.R.bn_ofint (Constants.q ^ (W64xN.valR res.`3) %% Constants.p), x) ] 
+   = Pr[ M1.commitment_indexed() @ &m : res.`1 = i /\ res.`3 = x ].
+have -> : Pr[ M1.commitment_indexed() @ &m : res.`1 = i /\ res.`3 = x ]
+ = Pr[ M1.commitment_indexed() @ &m : res.`1 = i /\ res.`3 = x 
+    /\ res.`2 = W64xN.R.bn_ofint (Constants.q ^ (W64xN.valR res.`3) %% Constants.p) ] + Pr[ M1.commitment_indexed() @ &m : res.`1 = i /\ res.`3 = x 
+    /\ res.`2 <> W64xN.R.bn_ofint (Constants.q ^ (W64xN.valR res.`3) %% Constants.p) ].
+rewrite Pr[mu_split (res.`2 = W64xN.R.bn_ofint (Constants.q ^ (W64xN.valR res.`3) %% Constants.p))]. smt().
+have ->:  Pr[ M1.commitment_indexed() @ &m : res.`1 = i /\ res.`3 = x 
+    /\ res.`2 <> W64xN.R.bn_ofint (Constants.q ^ (W64xN.valR res.`3) %% Constants.p) ] = 0%r. 
+   have : Pr[ M1.commitment_indexed() @ &m : res.`1 = i /\ res.`3 = x 
+    /\ res.`2 <> W64xN.R.bn_ofint (Constants.q ^ (W64xN.valR res.`3) %% Constants.p) ] <= Pr[ M1.commitment_indexed() @ &m : res.`2 <> W64xN.R.bn_ofint (Constants.q ^ (W64xN.valR res.`3) %% Constants.p) ]. rewrite Pr[mu_sub]. smt(). auto.
+  have ->: Pr[ M1.commitment_indexed() @ &m : res.`2 <> W64xN.R.bn_ofint (Constants.q ^ (W64xN.valR res.`3) %% Constants.p) ] = 0%r. rewrite commitment_cspec_pr2.
+auto. smt(@Distr). 
+simplify. rewrite Pr[mu_eq]. smt(). auto.
+qed.
+
+lemma commitment_cspec_pr i x &m :
+  Pr[ M1.commitment_indexed() @ &m : res.`1 = i /\ 
+   (res.`2, res.`3) = (W64xN.R.bn_ofint (Constants.q ^ (W64xN.valR res.`3) %% Constants.p), x)  ] 
+   = Pr[ CSpecFp.rsample(Constants.q) @ &m : res = (i, W64xN.valR x) ].
+rewrite commitment_cspec_pr3.
+rewrite commitment_cspec_pr1. auto.
+qed.
+
+lemma commitment_index_pos &m  : Pr[M1.commitment_indexed() @ &m : res.`1 <= 0 ] = 0%r.
+admitted.
+
+import W64xN.
+
+op g l : real 
+ = if inv (-1) commitment_t l <= 0 then 0%r else 
+     mu D (predC (RSP Constants.q)) ^ (inv (-1) commitment_t l - 1)
+       * (1%r / Ring_ops_spec.M%r).
+
+        
+lemma leakfree1 &m x l: (glob M1){m} = [] 
+  => Pr[ M1.commitment_indexed() @ &m : M1.leakages = l  /\ 
+   (res.`2, res.`3) = (W64xN.R.bn_ofint (Constants.q ^ (W64xN.valR x) %% Constants.p), x) ] 
+      = if W64xN.valR x < Constants.q then g l else 0%r.
+admitted.
+
+
+op h  : real = 1%r/Constants.q%r. 
+
+lemma leakfree2 &m x: 
+ Pr[ M1.commitment_indexed() @ &m : 
+   (res.`2, res.`3) = (W64xN.R.bn_ofint (Constants.q ^ (W64xN.valR x) %% Constants.p), x)  ] = if W64xN.valR x < Constants.q then h else 0%r. 
+admitted.
+
+op f l = h / g l.
+
+lemma commitment_indexed_leakfree l a &m: (glob M1){m} = [] 
+ =>  let v = Pr[ M1.commitment_indexed() @ &m : (res.`2, res.`3) = a  ] in 
+     let w = Pr[ M1.commitment_indexed() @ &m : M1.leakages = l  /\ (res.`2, res.`3) = a  ] in 
+  0%r < w => v/w 
+  = f  l.
+move => l_empty v w f1.
+
+pose a1_val := W64xN.R.bn_ofint (Constants.q ^ (W64xN.valR a.`2) %% Constants.p).  
+  
+have fact1 : a.`1 = a1_val.
+admit.
+have fact2 : valR a.`2 < Constants.q.
+admit.
+
+have -> : v = Pr[M1.commitment_indexed() @ &m : (res.`2, res.`3) = (a1_val, a.`2)].
+rewrite  /v Pr[mu_eq]. smt(). auto.
+have ->:  w = Pr[M1.commitment_indexed() @ &m :
+           M1.leakages = l /\ (res.`2, res.`3) = (a1_val, a.`2)].
+rewrite  /w Pr[mu_eq]. smt(). auto.
+
+rewrite /a1_val.
+
+rewrite (leakfree1 &m a.`2 l _).  auto.
+rewrite  (leakfree2 &m a.`2 ).  auto.
+
+rewrite fact2. simplify. auto.
+qed.
+
