proof/rejection_sampling/Ops_LeakageAnalysis.ec
@@ -1,0 +1,89 @@
+require import W64_SchnorrExtract_ct.
+require import List Int AllCore.
+
+from Jasmin require import JModel.
+
+(* SUBTRACTION LEAKAGES  *)
+op sub_prefix : leakages_t = 
+  [LeakFor (1, 32); LeakAddr []; LeakAddr [0]; LeakAddr []; 
+    LeakAddr []; LeakAddr [0]; LeakAddr [0]].
+
+op sub_step (i : int) : leakages_t = 
+  [LeakAddr [i] ; LeakAddr [] ; LeakAddr [] ; LeakAddr [i] ; 
+    LeakAddr [i] ].
+
+
+op sub_g (x : int) : leakages_t.
+axiom sub_g_comp_1 x : x <= 1 => sub_g x = [].
+axiom sub_g_comp_2 x : 1 <  x => sub_g x = sub_step (x-1) ++ sub_g (x - 1).
+
+op sub_f (x : int) : leakages_t = sub_g x ++ sub_prefix.
+
+
+lemma bn_subc_leakages start_l :
+  hoare [ M(Syscall).bn_subc : M.leakages = start_l 
+            ==> M.leakages = sub_f 32 ++ start_l ].
+proof. 
+proc.
+sp.  elim*. progress.
+conseq (_: M.leakages = sub_prefix ++ start_l /\ i = 1 ==> _).
+progress.
+while (0 < i /\ i <= 32 /\ M.leakages = sub_f i ++ start_l).
+wp.  skip.  progress. 
+simplify. smt(). smt(). rewrite /sub_f. rewrite (sub_g_comp_2 (i{hr} +1)).  smt(). simplify. rewrite /sub_step. simplify. auto.
+skip. progress. rewrite /sub_f.  rewrite sub_g_comp_1. auto. auto.
+smt().
+qed.
+
+
+(* COPY LEAKAGES  *)
+op copy_prefix : leakages_t = LeakFor (0, 32) :: LeakAddr [] ::[].
+op copy_step (i : int) : leakages_t = LeakAddr [i] :: LeakAddr [] :: LeakAddr [i] :: [].
+
+op copy_g (x : int) : leakages_t.
+axiom copy_g_comp_1 x : x <= 0 => copy_g x = [].
+axiom copy_g_comp_2 x : 0 <  x => copy_g x = copy_step (x-1) ++ copy_g (x - 1).
+
+op copy_f (x : int) : leakages_t = copy_g x ++ copy_prefix.
+
+lemma bn_copy_leakages start_l :
+   hoare [ M(Syscall).bn_copy : M.leakages = start_l 
+     ==> M.leakages = copy_f 32 ++ start_l ].
+proof. 
+proc.
+sp.  elim*. progress.
+conseq (_: M.leakages = copy_prefix ++ start_l /\ i = 0 ==> _).
+progress.
+while (0 <= i /\ i <= 32 /\ M.leakages = copy_f i ++ start_l).
+wp.  skip.  progress. 
+simplify. smt(). smt(). rewrite /copy_f. rewrite (copy_g_comp_2 (i{hr} +1)).  smt(). simplify. rewrite /copy_step. simplify. auto.
+skip. progress. rewrite /copy_f.  rewrite copy_g_comp_1. auto. auto. 
+smt().
+qed.
+
+
+
+(* set0 LEAKAGES  *)
+op set0_prefix : leakages_t = LeakFor (0, 32) :: LeakAddr [] :: [].
+op set0_step (i : int) : leakages_t = LeakAddr [i] :: LeakAddr [] :: [].
+
+op set0_g (x : int) : leakages_t.
+axiom set0_g_comp_1 x : x <= 0 => set0_g x = [].
+axiom set0_g_comp_2 x : 0 <  x => set0_g x = set0_step (x-1) ++ set0_g (x - 1).
+
+op set0_f (x : int) : leakages_t = set0_g x ++ set0_prefix.
+
+lemma bn_set0_leakages start_l :
+   hoare [ M(Syscall).bn_set0 : M.leakages = start_l 
+                ==> M.leakages = set0_f 32 ++ start_l ].
+proof. 
+proc.
+sp.  elim*. progress.
+conseq (_: M.leakages = set0_prefix ++ start_l /\ i = 0 ==> _).
+progress. rewrite /set0_prefix.
+while (0 <= i /\ i <= 32 /\ M.leakages = set0_f i ++ start_l).
+wp.  skip.  progress. 
+simplify. smt(). smt(). rewrite /set0_f. rewrite (set0_g_comp_2 (i{hr} +1)).  smt(). simplify. rewrite /set0_step. simplify. auto.
+skip. progress. rewrite /set0_f.  rewrite set0_g_comp_1. auto. auto. 
+smt().
+qed.
