proof/rejection_sampling/RejectionSamplingProperties.ec
@@ -29,6 +29,7 @@ lemma rs_lossless &m P1 c1 : mu d P1 > 0%r =>
 apply rj_lossless.
 qed.
 
+
 lemma rs_index &m P1 Q1 : 
  Impl Q1 P1 => forall i ,  0 <= i =>
   Pr[ RS.sample(P1,0) @ &m : Q1 res.`2 /\ res.`1 = i + 1 ] 
